AbsInterp.lean
@@ -6,7 +6,7 @@ import AbsInterp.Framework
 import AbsInterp.Framework.Concretization
 import AbsInterp.Framework.Domains
 import AbsInterp.Framework.Domains.Backward
-import AbsInterp.Framework.Domains.Gamma
+import AbsInterp.Framework.Domains.Concretization
 import AbsInterp.Framework.Domains.Interop.GaloisConnection
 import AbsInterp.Framework.Iteration
 import AbsInterp.Framework.Iteration.Collecting
