Tests.lean
@@ -2,10 +2,11 @@ import Cslib.Init
 
 import AbsInterp
 import Tests.Domains.Interval
+import Tests.Domains.Parity
 import Tests.Domains.Sign
 import Tests.Examples.IMP.Smoke
 import Tests.Examples.IMP.ParitySmoke
-import Tests.Framework.Domains.Gamma
+import Tests.Framework.Domains.Concretization
 import Tests.Instances.LTS.Smoke
 import Tests.Instances.LTS.Collecting
 import Tests.Instances.LTS.CollectingTrace
